Hs/Translator/Lemmas/TypesSoundness.lean
@@ -18,6 +18,39 @@ theorem is_type_list_reverse (τs : List Term) :
   replace h := h t lem
   assumption
 
+theorem hs_is_type_list_reverse (τs : List HsTerm) :
+  (∀ τ ∈ τs, HsTerm.IsType τ) -> ∀ τ ∈ τs.reverse, HsTerm.IsType τ := by
+  intro h t h2
+  have lem : t ∈ τs := by simp at h2; assumption
+  replace h := h t lem
+  assumption
+
+
+theorem hs_is_type_spine_application' (τh : HsTerm) (τs : List HsTerm) :
+  τh.IsType ->
+  (∀ τ ∈ τs, HsTerm.IsType τ) ->
+  HsTerm.IsType (τh.mk_kind_apps' τs) := by
+intro h1 h2; simp at *
+induction τs using List.foldr.induct <;> simp at *
+case _ => assumption
+case _ ih =>
+  cases h2; case _ h2a h2b =>
+  constructor;
+  replace ih := ih h2b; assumption
+  assumption
+
+
+theorem hs_is_type_spine_application (τh : HsTerm) (τs : List HsTerm) :
+  τh.IsType ->
+  (∀ τ ∈ τs, HsTerm.IsType τ) ->
+  HsTerm.IsType (τh.mk_kind_apps τs) := by
+intro h1 h2
+have lem := hs_is_type_list_reverse τs h2
+unfold HsTerm.mk_kind_apps
+apply hs_is_type_spine_application'
+assumption
+assumption
+
 
 theorem is_type_spine_application' (τh : Term) (τs : List Term) :
   τh.IsType ->
@@ -43,6 +76,13 @@ unfold Term.mk_kind_apps
 apply is_type_spine_application'
 assumption
 assumption
+
+theorem type_var_head_is_type_indexed {Γ : Ctx Term} {idx : Nat} {τ : HsTerm} :
+   ⊢ Γ ->
+   τ.IsType ->
+   τ.neutral_form = .some (`#idx, sp) ->
+   Γ d@ idx = (Frame.type τ') := by sorry
+
 
 theorem compile_type_shape_soundness (Γ : Ctx Term) (k : Term) (τ : HsTerm) (τ' : Term): ⊢ Γ ->
  HsTerm.IsType τ ->
@@ -103,47 +143,56 @@ case _ sp idx _ tnfp _ _ _ _ =>
     have e := Term.eq_of_beq j6; cases e; clear j6
     cases j3; case _ exp_κ τ _ _ _ _ _ j3 j6 =>
     cases j6;
+    rw[List.foldl_eq_foldr_reverse]
     have lem1 := HsTerm.hs_type_neutral_form_is_type j1 tnfp
     have lem2 := HsTerm.hs_is_type_neutral_form j1 tnfp
+    rw[<-List.mapM'_eq_mapM] at j3
     cases lem1; case _ lem1a =>
-    -- have κ_wf : κ.IsKind := by sorry
-    -- have lem3 := kind_shape_split_arrow κ_wf j4
-    -- cases lem3; case _ lem3a lem3b =>
-    rw[List.foldl_eq_foldr_reverse]
+    have κ_wf : κ.IsKind := by sorry
+    have lem3 := kind_shape_split_arrow κ_wf j4
+    cases lem3; case _ lem3a lem3b =>
     apply is_type_spine_application
     case _ => constructor
     case _ ih _ _ =>
-      intro sp_τ τ_in_sp
-      induction [], κ using Term.split_kind_arrow_aux.induct <;> simp at j4
-      sorry
+      intro τ' τ'_in_τs
+      have lem3 := mapM'_elems_image j3 τ' τ'_in_τs
+      cases lem3; case _ lem3 =>
+      cases lem3; case _ w w_in_sp lem3 =>
+      simp at lem3; split at lem3 <;> simp at lem3
+      case _ contra => simp at contra
+      case _ e _ =>
+        have lem2' := lem2 (w.val.snd.val.fst, w.val.snd.val.snd) w.val.snd.property
+        simp at lem2'; cases lem2'
+        apply ih κs w.val.fst w.val.fst.property (w.val.snd.val.fst) _ _ _ τ' wf _ _ lem3
+        apply w.val.snd.property
+        apply w.property
+        assumption
+        apply lem3b w.val.fst.val w.val.fst.property
+      case _ contra => simp at contra
+
+
+
+      -- induction [], κ using Term.split_kind_arrow_aux.induct generalizing κs sp <;> simp at j4
       -- have ih' := ih κs
-      case _ =>
-        cases j4.1; cases j4.2; simp at j3; cases j3; cases τ_in_sp
+      -- sorry
+      -- case _ =>
+      --   cases j4.1; cases j4.2; simp at j3; cases j3; cases τ_in_sp
 
-    -- generalize zzh : κs.attach.zip sp.attach = zz at *
-    -- induction κs generalizing sp <;> simp at zzh
-    -- case _ =>
-    --   cases zzh
-    --   simp at j3; unfold pure at j3; unfold Applicative.toPure at j3;
-    --   unfold Monad.toApplicative at j3; unfold Except.instMonad at j3; simp at j3;
-    --   unfold Except.pure at j3; simp at j3; cases j3; simp; constructor
-    -- case _ κhd κtl _ _ =>
-    --   induction sp <;> simp at zzh
-    --   case _ =>
-    --     cases zzh
-    --     simp at j3; unfold pure at j3; unfold Applicative.toPure at j3;
-    --     unfold Monad.toApplicative at j3; unfold Except.instMonad at j3; simp at j3;
-    --     unfold Except.pure at j3; simp at j3; cases j3; simp; constructor
-    --   case _ sph sptl _ _ =>
-    --     rw[<-zzh] at j3; rw[<-List.mapM'_eq_mapM] at j3
-    --     simp at j3
-    --     unfold bind at j3; unfold Monad.toBind at j3; unfold Except.instMonad at j3; simp at j3
-    --     cases j3; case _ j3 =>
-    --     cases j3; case _ j3a j3b =>
-    --     simp at j3a; simp at j3b
-    --     unfold Except.map at j3b; split at j3b <;> simp at j3b
-    --     cases j3b; rw[List.foldl_eq_foldr_reverse]; sorry
-
+      -- generalize zzh : κs.attach.zip sp.attach = zz at *
+      -- induction κs generalizing sp <;> simp at zzh
+      -- case _ => cases zzh; cases j3; simp at τ'_in_sp
+      -- case _ κhd κtl _ _ =>
+      --   induction sp <;> simp at zzh
+      --   case _ => cases zzh; simp at j3; cases j3; sorry
+      --   case _ sph sptl _ _ =>
+      --     rw[<-zzh] at j3; rw[<-List.mapM'_eq_mapM] at j3
+      --     simp at j3
+      --     unfold bind at j3; unfold Monad.toBind at j3; unfold Except.instMonad at j3; simp at j3
+      --     cases j3; case _ j3 =>
+      --     cases j3; case _ j3a j3b =>
+      --     simp at j3a; simp at j3b
+      --     unfold Except.map at j3b; split at j3b <;> simp at j3b
+      --     cases j3b; sorry
 
 
 
